A more sensible way to prove correctness of the Arity Analysis

Launchbury/ArityCorrectSestoft.thy
@@ -2,11 +2,95 @@ theory ArityCorrectSestoft
 imports ArityCorrect SestoftCorrect
 begin
 
-fun stack_arity :: "stack \<Rightarrow> Arity"
-  where "stack_arity [] = 0"
-      | "stack_arity (Arg x # S) = inc_Arity (stack_arity S)"
-      | "stack_arity (Upd x # S) = stack_arity S"
-      | "stack_arity (Dummy x # S) = stack_arity S"
+fun Astack :: "AEnv \<Rightarrow> stack \<Rightarrow> Arity"
+  where "Astack ae [] = 0"
+      | "Astack ae (Arg x # S) = inc\<cdot>(Astack ae S)"
+      | "Astack ae (Upd x # S) = (case ae x of Iup a \<Rightarrow> a)"
+      | "Astack ae (Dummy x # S) = 0"
+
+lemma Astack_Upd_simps[simp]:
+  "ae x = up\<cdot>u \<Longrightarrow> Astack ae (Upd x # S) = u"
+  by (simp add: up_def cont_Iup)
+declare Astack.simps(3)[simp del]
+
+fun AEstack :: "AEnv \<Rightarrow> stack \<Rightarrow> AEnv"
+  where "AEstack ae [] = \<bottom>"
+      | "AEstack ae (Arg x # S) = AE_singleton x \<cdot> (up\<cdot>0) \<squnion> AEstack ae S"
+      | "AEstack ae (Upd x # S) = AE_singleton x \<cdot> (up\<cdot>(Astack ae S)) \<squnion> AEstack ae S"
+      | "AEstack ae (Dummy x # S) = AEstack ae S"
+
+context CorrectArityAnalysis
+begin
+
+inductive AE_consistent :: "AEnv \<Rightarrow> conf \<Rightarrow> bool" where
+  AE_consistentI: 
+  "upds S \<subseteq> edom ae
+  \<Longrightarrow> AEstack ae S \<sqsubseteq> ae 
+  \<Longrightarrow> Aexp e \<cdot> (Astack ae S) \<sqsubseteq> ae
+  \<Longrightarrow> (\<And> x e. map_of \<Gamma> x = Some e \<Longrightarrow> Aexp' e \<cdot> (ae x) \<sqsubseteq> ae)
+  \<Longrightarrow> AE_consistent ae (\<Gamma>, e, S)"
+
+inductive_cases AE_consistentE[elim]: "AE_consistent ae (\<Gamma>, e, S)"
+
+lemma [simp]: "Aexp' e\<cdot>(Iup u) = Aexp e\<cdot>u"
+proof-
+  have "Iup u = up\<cdot>u" by (simp add: up_def cont_Iup )
+  thus ?thesis by simp
+qed
+
+lemma map_of_deleteD: "map_of (delete x \<Gamma>) xa = Some e \<Longrightarrow> map_of \<Gamma> xa = Some e"
+  by (metis delete_conv fun_upd_same map_of_delete option.distinct(1))
+
+theorem
+  assumes "(\<Gamma>, e, S) \<Rightarrow> (\<Delta>, v, S')"
+  assumes "AE_consistent ae (\<Gamma>, e, S)"
+(*   shows "AE_consistent ae (\<Delta>, v, S')" *)
+  shows "\<exists> ae'. ae' f|` (-((domA \<Delta> \<union> upds S') - (domA \<Gamma> \<union> upds S))) = ae \<and> AE_consistent ae' (\<Delta>, v, S')"
+using assms
+proof(induction "(\<Gamma>, e, S)" "(\<Delta>, v, S')"  arbitrary: \<Gamma> e S \<Delta> v S' rule: step.inducts)
+case (app\<^sub>1 \<Gamma> e x S)
+  hence "AE_consistent ae (\<Gamma>, e, Arg x # S)"  by (fastforce elim!: AE_consistentE intro!: AE_consistentI simp add: Aexp_App join_below_iff)
+  thus ?case by simp
+next
+case (app\<^sub>2 \<Gamma> y e x S)
+  hence "AE_consistent ae (\<Gamma>, e[y::=x], S)" 
+    by (auto elim!: AE_consistentE intro!: AE_consistentI  below_trans[OF monofun_cfun_fun[OF Aexp_subst_App_Lam]] simp add: Aexp_App join_below_iff)
+  thus ?case by simp
+next
+case (var\<^sub>1 \<Gamma> x e S)
+  from `map_of \<Gamma> x = Some e`
+  have "x \<in> domA \<Gamma>" by (metis domI dom_map_of_conv_domA)
+  hence *: "(domA (delete x \<Gamma>) \<union> upds (Upd x # S) - (domA \<Gamma> \<union> upds S)) = {}" using `x \<in> domA \<Gamma>` by auto
+  
+  from var\<^sub>1 have "Aexp (Var x)\<cdot>(Astack ae S) \<sqsubseteq> ae" by auto
+  from below_trans[OF Aexp_Var fun_belowD[OF this] ]
+  have "up\<cdot>(Astack ae S) \<sqsubseteq> ae x".
+  then obtain u where "ae x = up\<cdot>u" and "Astack ae S \<sqsubseteq> u" by (cases "ae x") auto
+  moreover
+  hence "x \<in> edom ae" unfolding edom_def by auto
+  ultimately
+  have "AE_consistent ae (delete x \<Gamma>, e, Upd x # S)" using var\<^sub>1 by (fastforce intro!: AE_consistentI dest: map_of_deleteD simp add: join_below_iff)
+  thus ?case unfolding * by simp
+next
+case (var\<^sub>2 x \<Gamma> e S)
+  have "up\<cdot>(Astack ae S) \<sqsubseteq> ae x" using var\<^sub>2 by (auto simp add: join_below_iff)
+  then obtain u where "ae x = up \<cdot> u" and "Astack ae S \<sqsubseteq> u" by (cases "ae x") auto
+
+  from this(2)
+  have "Aexp e\<cdot>(Astack ae S) \<sqsubseteq> Aexp e\<cdot>u" by (rule monofun_cfun_arg)
+  also have "\<dots> \<sqsubseteq> ae" using `ae x = up \<cdot> u` var\<^sub>2 by auto
+  finally have "Aexp e\<cdot>(Astack ae S) \<sqsubseteq> ae" by this simp
+  hence "AE_consistent ae ((x, e) # \<Gamma>, e, S)" using var\<^sub>2 `ae x = up \<cdot> u`
+    by (fastforce intro!: AE_consistentI  simp add: join_below_iff split:if_splits)+
+  thus ?case by simp
+next
+case (let\<^sub>1 x \<Gamma> e S)
+  show ?case
+    sorry
+qed
+
+
+(*
 
 nominal_function maybeVar :: "exp \<Rightarrow> var option" where
   "maybeVar (Var x) = Some x" |
@@ -34,12 +118,12 @@ context CorrectArityAnalysis
 begin
 
 fun  conf_analysis :: "conf \<Rightarrow> AEnv"
-where "conf_analysis (\<Gamma>,e,S) =  Afix \<Gamma>\<cdot>(Aexp e\<cdot>(stack_arity S))" 
+where "conf_analysis (\<Gamma>,e,S) = Afix \<Gamma>\<cdot>(Aexp e\<cdot>(stack_arity S))" 
 lemmas conf_analysis.simps[simp del]
 
 lemma arity_preservation:
   assumes "(\<Gamma>, e, S) \<Rightarrow> (\<Gamma>', e', S')"
-  shows "conf_analysis (\<Gamma>', e', S') \<sqsubseteq> conf_analysis (\<Gamma>, e, S)"
+  shows "conf_analysis (\<Gamma>', e', S')  f|` (- (domA \<Gamma>' - domA \<Gamma>))  \<sqsubseteq> conf_analysis (\<Gamma>, e, S)  f|` (- (domA \<Gamma>' - domA \<Gamma>)) "
 sorry
 
 lemma arity_correct_now:
@@ -54,8 +138,8 @@ case goal1
 qed auto
 
 theorem
-  assumes "(\<Gamma>, e, S) \<Rightarrow>\<^sup>*\<^bsub>T\<^esub> final"
-  shows "trace_arities ((\<Gamma>, e, S) # T) \<sqsubseteq> conf_analysis (\<Gamma>, e, S)"
+  assumes "(\<Gamma>, e, S) \<Rightarrow>\<^sup>*\<^bsub>T\<^esub> (\<Delta>, v, S')"
+  shows "trace_arities ((\<Gamma>, e, S) # T) f|` (- (domA \<Delta> - domA \<Gamma>)) \<sqsubseteq> conf_analysis (\<Gamma>, e, S)  f|` (- (domA \<Delta> - domA \<Gamma>))"
 using assms
 proof(induction rule: conf_trace_induct_final)
   case (trace_nil \<Gamma> e S)
@@ -63,15 +147,26 @@ proof(induction rule: conf_trace_induct_final)
 next
   case (trace_cons \<Gamma> e S T \<Gamma>' e' S')
 
-  have "conf_arities (\<Gamma>, e, S) \<sqsubseteq> conf_analysis (\<Gamma>, e, S)" by (rule arity_correct_now)
+  have "domA \<Gamma> \<subseteq> domA \<Gamma>'" and "domA \<Gamma>' \<subseteq> domA \<Delta>" sorry
+  hence subset1: "- (domA \<Delta> - domA \<Gamma>) \<subseteq> - (domA \<Delta> - domA \<Gamma>')" and
+        subset2: "- (domA \<Delta> - domA \<Gamma>) \<subseteq> - (domA \<Gamma>' - domA \<Gamma>)" by auto
+
+  from arity_correct_now
+  have "conf_arities (\<Gamma>, e, S)  f|` (- (domA \<Delta> - domA \<Gamma>)) \<sqsubseteq> conf_analysis (\<Gamma>, e, S)  f|` (- (domA \<Delta> - domA \<Gamma>))" by (rule env_restr_mono)
   moreover
-  note `trace_arities ((\<Gamma>', e', S') # T) \<sqsubseteq> conf_analysis (\<Gamma>', e', S')`
+  from trace_cons(3)
+  have "trace_arities ((\<Gamma>', e', S') # T)  f|` (- (domA \<Delta> - domA \<Gamma>)) \<sqsubseteq> conf_analysis (\<Gamma>', e', S')  f|` (- (domA \<Delta> - domA \<Gamma>))"
+    by (rule env_restr_below_subset[OF subset1])
   moreover
   from `(\<Gamma>, e, S) \<Rightarrow> (\<Gamma>', e', S')`
-  have "conf_analysis (\<Gamma>', e', S') \<sqsubseteq> conf_analysis (\<Gamma>, e, S)"
+  have "conf_analysis (\<Gamma>', e', S')  f|` (- (domA \<Gamma>' - domA \<Gamma>)) \<sqsubseteq> conf_analysis (\<Gamma>, e, S)  f|` (- (domA \<Gamma>' - domA \<Gamma>))"
     by (rule arity_preservation)
+  hence "conf_analysis (\<Gamma>', e', S')  f|` (- (domA \<Delta> - domA \<Gamma>)) \<sqsubseteq> conf_analysis (\<Gamma>, e, S)  f|` (- (domA \<Delta> - domA \<Gamma>))"
+    by (rule env_restr_below_subset[OF subset2])
   ultimately
-  show ?case by (auto intro: join_below dest: below_trans simp del: conf_arities.simps fun_meet_simp)
+  show ?case by (auto intro: join_below dest: below_trans simp add: env_restr_join simp del: conf_arities.simps fun_meet_simp)
 qed
+
+*)
 
 end
